Logics.lean
@@ -4,6 +4,7 @@ import Logics.Lattice
 import Logics.Heyting
 import Logics.Lindenbaum
 import Logics.Homomorphism
+import Logics.FiniteFrame
 import Logics.ConcreteEmbed
 import Logics.Filter
 import Logics.Jankov
